specs/Spec.Tree.Lemmas.fst
@@ -1,0 +1,1029 @@
+module Spec.Tree.Lemmas
+
+open FStar.Mul
+
+let lemma_subtraction_cancel (a b c: int): Lemma
+  (requires b = a - c)
+  (ensures b + c == a) = ()
+
+#set-options "--z3refresh --z3rlimit 256 --fuel 0 --ifuel 0"
+let lemma_heap_seq (ts: heap_wf_ts) (i: heap_index ts): Lemma
+  (requires i <= ts.heap_len)
+  (ensures
+    (element_seq ts).[i - 1] == ts.heap.[i] /\
+    (heap_seq ts).[i - 1] == ts.heap.[i]) =
+  let es = element_seq ts in
+  let i' = i - 1 in
+  assert(forall (j: nat). {:pattern es.[j]} j < ts.heap_len ==>
+    ts.heap.[j + 1] == es.[j]);
+  assert(es.[i'] == ts.heap.[i' + 1]);
+  lemma_subtraction_cancel i i' 1
+
+let lemma_sorted_seq (ts: heap_wf_ts) (i: heap_index ts): Lemma
+  (requires i >= ts.heap_max)
+  (ensures
+    (element_seq ts).[i - (ts.heap_max - ts.heap_len)] == ts.heap.[i] /\
+    (sorted_seq ts).[i - ts.heap_max] == ts.heap.[i]) =
+  let es = element_seq ts in
+  let i' = i - (ts.heap_max - ts.heap_len) in
+  assert(forall j. {:pattern es.[j]} j >= ts.heap_len ==>
+    ts.heap.[j - ts.heap_len + ts.heap_max] == es.[j]);
+  assert(es.[i'] == ts.heap.[i' + (ts.heap_max - ts.heap_len)]);
+  lemma_subtraction_cancel i i' (ts.heap_max - ts.heap_len)
+
+let lemma_pqremove_index
+  (ts: forest_wf_ts{ts.heap_len > 1})
+  (i: heap_index (pqremove ts)): Lemma
+  (ensures (
+    let ts' = pqremove ts in
+    (mem ts'.heap.[i] (element_seq ts')) /\
+    ((exists j. (heap_seq ts).[j] == ts'.heap.[i]) \/
+    (exists j. (sorted_seq ts).[j] == ts'.heap.[i])))) =
+  let ts' = pqremove ts in
+  let es' = element_seq ts' in
+  if i <= ts'.heap_len then
+    lemma_heap_seq ts' i
+  else
+    lemma_sorted_seq ts' i;
+  assert(mem ts'.heap.[i] es');
+  assert(mem ts'.heap.[i] (element_seq ts));
+  lemma_mem_append (heap_seq ts) (sorted_seq ts);
+  if mem ts'.heap.[i] (heap_seq ts) then
+    mem_index ts'.heap.[i] (heap_seq ts)
+  else
+    mem_index ts'.heap.[i] (sorted_seq ts)
+
+#set-options "--z3refresh --z3rlimit 1024 --fuel 0 --ifuel 0"
+let lemma_pqremove_forest_aux
+  (ts: forest_wf_ts{ts.heap_len > 1})
+  (i: heap_index (pqremove ts)): Lemma
+  (requires (
+    let ts' = pqremove ts in
+    ts'.heap_max < i))
+  (ensures (
+    let ts' = pqremove ts in
+    let (es, es') = (element_seq ts, element_seq ts') in
+    let dad = Cast.uint16_to_uint32 (ts'.tree.[U32.v ts'.heap.[i]]).dad_or_len in
+    mem ts'.heap.[i] es /\
+    i - (ts'.heap_max - ts'.heap_len) == index_of es ts'.heap.[i] /\
+    mem dad es)) =
+  lemma_pqremove_index ts i;
+  let ts' = pqremove ts in
+  let (es, es') = (element_seq ts, element_seq ts') in
+  let j = index_of es ts'.heap.[i] in
+  let i' = i - (ts'.heap_max - ts'.heap_len) in
+  let j' = j + (ts.heap_max - ts.heap_len) in
+  lemma_sorted_seq ts' i;
+  no_dup_index_of es i' ts'.heap.[i];
+  no_dup_index_of es' j ts'.heap.[i];
+  lemma_sorted_seq ts j';
+
+  lemma_sorted_seq ts i;
+  lemma_sorted_seq ts' i;
+  assert(tree_corr ts i /\ parent_corr ts i);
+  assert(ts.heap_max <= i /\ ts'.heap.[i] == ts.heap.[i])
+
+#push-options "--fuel 1 --ifuel 1"
+let rec lemma_forest_symbols_append
+  (ts: heap_elems_wf_ts) (s0 s1: tree_id_seq ts): Lemma
+  (ensures forest_symbols ts s0 @| forest_symbols ts s1 == forest_symbols ts (s0 @| s1))
+  (decreases length s0) =
+  match length s0 with
+  | 0 ->
+    calc (==) {
+      forest_symbols ts s0 @| forest_symbols ts s1;
+      =={}
+      empty #nat @| forest_symbols ts s1;
+      =={append_empty_l (forest_symbols ts s1)}
+      forest_symbols ts s1;
+      =={
+        lemma_empty s0;
+        append_empty_l s1
+      }
+      forest_symbols ts (s0 @| s1);
+    }
+  | _ ->
+    calc (==) {
+      forest_symbols ts s0 @| forest_symbols ts s1;
+      =={}
+      (symbols ts.forest.[U32.v s0.[0]] @| forest_symbols ts (tail s0)) @|
+      forest_symbols ts s1;
+      =={
+        append_assoc
+          (symbols ts.forest.[U32.v s0.[0]])
+          (forest_symbols ts (tail s0))
+          (forest_symbols ts s1)
+      }
+      symbols ts.forest.[U32.v s0.[0]] @|
+      (forest_symbols ts (tail s0) @| forest_symbols ts s1);
+      =={lemma_forest_symbols_append ts (tail s0) s1}
+      symbols ts.forest.[U32.v s0.[0]] @| forest_symbols ts ((tail s0) @| s1);
+      =={assert(((tail s0) @| s1) `equal` (tail (s0 @| s1)))}
+      symbols ts.forest.[U32.v s0.[0]] @| forest_symbols ts (tail (s0 @| s1));
+      =={}
+      forest_symbols ts (s0 @| s1);
+    }
+
+#push-options "--fuel 0 --ifuel 0"
+let lemma_forest_symbols_middle
+  (ts: heap_elems_wf_ts) (s: tree_id_seq ts) (i: index_t s) (n: nat): Lemma
+  (ensures
+    count n (forest_symbols ts (slice s 0 i)) +
+    count n (forest_symbols ts (create 1 s.[i])) +
+    count n (forest_symbols ts (slice s (i + 1) (length s))) =
+    count n (forest_symbols ts s)) =
+  calc (==) {
+    count n (forest_symbols ts s);
+    =={slice_middle s i}
+    count n (forest_symbols ts (
+      slice s 0 i @|
+      create 1 s.[i] @|
+      slice s (i + 1) (length s)));
+    =={append_assoc (slice s 0 i) (create 1 s.[i]) (slice s (i + 1) (length s))}
+    count n (forest_symbols ts ((
+      slice s 0 i @|
+      create 1 s.[i]) @|
+      slice s (i + 1) (length s)));
+    =={
+      lemma_forest_symbols_append ts
+        (slice s 0 i @| create 1 s.[i])
+        (slice s (i + 1) (length s))
+    }
+    count n (
+      (forest_symbols ts (slice s 0 i @| create 1 s.[i])) @|
+      (forest_symbols ts (slice s (i + 1) (length s))));
+    =={lemma_forest_symbols_append ts (slice s 0 i) (create 1 s.[i])}
+    count n (
+      ((forest_symbols ts (slice s 0 i)) @|
+      (forest_symbols ts (create 1 s.[i]))) @|
+      (forest_symbols ts (slice s (i + 1) (length s))));
+    =={
+      lemma_append_count_aux n
+        (forest_symbols ts (slice s 0 i) @| forest_symbols ts (create 1 s.[i]))
+        (forest_symbols ts (slice s (i + 1) (length s)))
+    }
+    count n (forest_symbols ts (slice s 0 i) @| forest_symbols ts (create 1 s.[i])) +
+    count n (forest_symbols ts (slice s (i + 1) (length s)));
+    =={
+      lemma_append_count_aux n
+        (forest_symbols ts (slice s 0 i))
+        (forest_symbols ts (create 1 s.[i]))
+    }
+    count n (forest_symbols ts (slice s 0 i)) +
+    count n (forest_symbols ts (create 1 s.[i])) +
+    count n (forest_symbols ts (slice s (i + 1) (length s)));
+  }
+#pop-options
+  
+#push-options "--fuel 2 --ifuel 2"
+let lemma_forest_symbols_single
+  (ts: heap_elems_wf_ts) (s: U32.t{is_tree_index ts s}): Lemma
+  (ensures symbols ts.forest.[U32.v s] == forest_symbols ts (create 1 s)) = ()
+#pop-options
+
+#push-options "--z3seed 1 --fuel 1 --ifuel 0"
+let rec lemma_forest_symbols_perm_aux
+  (ts0: heap_elems_wf_ts) (s0: tree_id_seq ts0)
+  (ts1: heap_elems_wf_ts) (s1: tree_id_seq ts1)
+  (s: nat): Lemma
+  (requires ts0.forest == ts1.forest /\ permutation U32.t s0 s1)
+  (ensures count s (forest_symbols ts0 s0) == count s (forest_symbols ts1 s1))
+  (decreases length s0) =
+  match length s0 with
+  | 0 -> ()
+  | _ ->
+    let i = index_of s1 s0.[0] in
+    let hd0 = symbols ts0.forest.[U32.v s0.[0]] in
+    let hd1 = symbols ts1.forest.[U32.v s1.[i]] in
+    let s1' = slice s1 0 i @| slice s1 (i + 1) (length s1) in
+    perm_len s0 s1;
+    calc (==) {
+      count s (forest_symbols ts0 s0);
+      =={}
+      count s (hd1 @| forest_symbols ts0 (tail s0));
+      =={lemma_append_count_aux s hd1 (forest_symbols ts0 (tail s0))}
+      count s hd1 + count s (forest_symbols ts0 (tail s0));
+      =={
+        permutation_middle s0 s1;
+        lemma_forest_symbols_perm_aux ts0 (tail s0) ts1 s1' s
+      }
+      count s hd1 + count s (forest_symbols ts1 s1');
+      =={
+        lemma_forest_symbols_append ts1
+          (slice s1 0 i)
+          (slice s1 (i + 1) (length s1))
+      }
+      count s hd1 +
+      count s (
+        forest_symbols ts1 (slice s1 0 i) @|
+        forest_symbols ts1 (slice s1 (i + 1) (length s1)));
+      =={
+        lemma_append_count_aux s
+          (forest_symbols ts1 (slice s1 0 i))
+          (forest_symbols ts1 (slice s1 (i + 1) (length s1)))
+      }
+      count s (forest_symbols ts1 (slice s1 0 i)) +
+      count s hd1 +
+      count s (forest_symbols ts1 (slice s1 (i + 1) (length s1)));
+      =={lemma_forest_symbols_single ts1 s1.[i]}
+      count s (forest_symbols ts1 (slice s1 0 i)) +
+      count s (forest_symbols ts1 (create 1 s1.[i])) +
+      count s (forest_symbols ts1 (slice s1 (i + 1) (length s1)));
+      =={lemma_forest_symbols_middle ts1 s1 i s}
+      count s (forest_symbols ts1 s1);
+    }
+
+let lemma_forest_symbols_perm ts0 s0 ts1 s1 =
+  let open FStar.Classical in
+  forall_intro (move_requires (lemma_forest_symbols_perm_aux ts0 s0 ts1 s1))
+#pop-options
+
+let lemma_is_max_id_map ts node i =
+  let es = element_seq ts in
+  if i <= ts.heap_len then
+    lemma_heap_seq ts i
+  else
+    lemma_sorted_seq ts i;
+  mem_index ts.heap.[i] es
+
+#push-options "--fuel 2 --ifuel 2"
+let lemma_pqremove_child_corr
+  (ts: forest_wf_ts{ts.heap_len > 1})
+  (i: heap_index (pqremove ts)): Lemma
+  (ensures 
+    // let ts' = pqremove ts in
+    // id ts'.forest.[U32.v ts'.heap.[i]] == U32.v ts'.heap.[i] /\
+    child_corr (pqremove ts) i) =
+  let ts' = pqremove ts in
+  let i' = U32.v ts'.heap.[i] in
+  let t = ts'.forest.[i'] in
+  lemma_pqremove_index ts i;
+  if Node? t then begin
+    assert(ts.forest.[i'] == t);
+    let l = id (left t) in let r = id (right t) in
+    assert(l < id t /\ r < id t);
+    assert(exists (j: heap_index ts). ts.heap.[j] == ts'.heap.[i] /\ child_corr ts j)
+  end
+#pop-options
+
+#push-options "--z3seed 1"
+let lemma_pqremove_heap_seq_index
+  (ts: forest_wf_ts{ts.heap_len > 1})
+  (i: index_t (element_seq ts)): Lemma
+  (requires 0 < i /\ i < ts.heap_len)
+  (ensures (
+    let ts' = pqremove ts in
+    index_of (element_seq ts') (element_seq ts).[i] < ts'.heap_len)) =
+  let ts' = pqremove ts in
+  let es = element_seq ts in
+  let es' = element_seq ts' in
+  if index_of es' es.[i] = ts'.heap_len then
+    no_dup_alt es i 0
+  else if ts'.heap_len < index_of es' es.[i] then
+    calc (==) {
+      count es.[i] es';
+      =={
+        calc (==) {
+          es';
+          =={}
+          heap_seq ts' @| sorted_seq ts';
+          =={assert(equal (cons es.[0] (sorted_seq ts)) (sorted_seq ts'))}
+          heap_seq ts' @| cons es.[0] (sorted_seq ts);
+          =={}
+          heap_seq ts' @| (create 1 es.[0] @| sorted_seq ts);
+          =={append_assoc (heap_seq ts') (create 1 es.[0]) (sorted_seq ts)}
+          (heap_seq ts' @| create 1 es.[0]) @| sorted_seq ts;
+        }
+      }
+      count es.[i] ((heap_seq ts' @| create 1 es.[0]) @| sorted_seq ts);
+      =={lemma_append_count_aux es.[i] (heap_seq ts' @| create 1 es.[0]) (sorted_seq ts)}
+      count es.[i] (heap_seq ts' @| create 1 es.[0]) + count es.[i] (sorted_seq ts);
+      =={lemma_append_count_aux es.[i] (heap_seq ts) (sorted_seq ts)}
+      count es.[i] (heap_seq ts) + count es.[i] (sorted_seq ts);
+    }
+  else
+    assert(index_of es' es.[i] < ts'.heap_len)
+#pop-options
+
+#push-options "--z3seed 0 --fuel 0 --ifuel 0 --query_stats"
+let lemma_pqremove_forest'
+  (ts: forest_wf_ts{ts.heap_len > 1})
+  (i: heap_index (pqremove ts)): Lemma
+  (ensures (
+    let ts' = pqremove ts in
+    freq_corr ts' i /\
+    id ts'.forest.[U32.v ts'.heap.[i]] == U32.v ts'.heap.[i] /\
+    (ts'.heap_max == i ==> child_corr ts' i) /\
+    (ts'.heap_max <> i ==> tree_corr ts' i))) =
+  lemma_pqremove_index ts i;
+  lemma_pqremove_child_corr ts i;
+  let ts' = pqremove ts in
+  let es = element_seq ts in
+  let es' = element_seq ts' in
+  let j = index_of es ts'.heap.[i] in
+  let dad = Cast.uint16_to_uint32 (ts'.tree.[U32.v ts'.heap.[i]]).dad_or_len in
+  assert(exists (j: heap_index ts). ts.heap.[j] == ts'.heap.[i] /\ freq_corr ts j);
+  if ts'.heap_max < i then begin
+    lemma_pqremove_forest_aux ts i;
+    lemma_sorted_seq ts (j + (ts.heap_max - ts.heap_len));
+    let k = index_of es dad in
+    if ts.heap_len <= k then () else if k = 0 then
+      no_dup_index_of es' ts'.heap_len dad
+    else
+      lemma_pqremove_heap_seq_index ts k
+  end
+#pop-options
+
+let lemma_pqremove_id'
+  (ts: forest_wf_ts{ts.heap_len > 1})
+  (node: nat{is_max_id ts node})
+  (i: index_t (element_seq ts)): Lemma
+  (ensures id (pqremove ts).forest.[U32.v (element_seq (pqremove ts)).[i]] < node) =
+  let ts' = pqremove ts in
+  let (es, es') = (element_seq ts, element_seq ts') in
+  count_index es';
+  mem_index es'.[i] es
+
+#push-options "--z3seed 6 --fuel 0 --ifuel 0 --query_stats"
+let lemma_pqremove_id
+  (ts: forest_wf_ts{ts.heap_len > 1}) (node: nat{is_max_id ts node}): Lemma
+  (ensures is_max_id (pqremove ts) node) =
+  FStar.Classical.forall_intro (lemma_pqremove_id' ts node);
+  perm_len (element_seq ts) (element_seq (pqremove ts))
+#pop-options
+
+#push-options "--fuel 1 --ifuel 1"
+let rec lemma_forest_freq_unsnoc (ts: heap_elems_wf_ts) (s: tree_id_seq ts): Lemma
+  (requires length s > 0)
+  (ensures
+    forest_freq ts s ==
+    forest_freq ts (unsnoc s) + freq ts.forest.[U32.v (last s)])
+  (decreases length s) =
+  match length s with
+  | 1 -> ()
+  | _ ->
+    assert(cons s.[0] (unsnoc (tail s)) `equal` unsnoc s);
+    lemma_forest_freq_unsnoc ts (tail s)
+
+let rec lemma_forest_freq_middle
+  (ts: heap_elems_wf_ts) (s: tree_id_seq ts) (i: index_t s): Lemma
+  (requires length s > 0)
+  (ensures forest_freq ts s ==
+    forest_freq ts (slice s 0 i) +
+    freq ts.forest.[U32.v s.[i]] +
+    forest_freq ts (slice s (i + 1) (length s)))
+  (decreases i) =
+  if i > 0 then lemma_forest_freq_middle ts (tail s) (i - 1)
+
+let rec lemma_forest_freq_append
+  (ts: heap_elems_wf_ts) (s0 s1: tree_id_seq ts): Lemma
+  (ensures forest_freq ts s0 + forest_freq ts s1 == forest_freq ts (s0 @| s1))
+  (decreases length s0) =
+  match length s0 with
+  | 0 ->
+    calc (==) {
+      forest_freq ts s0 + forest_freq ts s1;
+      =={}
+      forest_freq ts s1;
+      =={
+        lemma_empty s0;
+        append_empty_l s1
+     }
+     forest_freq ts (s0 @| s1);
+    }
+  | _ ->
+    calc (==) {
+      forest_freq ts s0 + forest_freq ts s1;
+      =={}
+      freq ts.forest.[U32.v s0.[0]] + (forest_freq ts (tail s0) + forest_freq ts s1);
+      =={lemma_forest_freq_append ts (tail s0) s1}
+      freq ts.forest.[U32.v s0.[0]] + forest_freq ts ((tail s0) @| s1);
+      =={assert(((tail s0) @| s1) `equal` tail (s0 @| s1))}
+      freq ts.forest.[U32.v s0.[0]] + forest_freq ts (tail (s0 @| s1));
+      =={}
+      forest_freq ts (s0 @| s1);
+    }
+
+let rec lemma_forest_freq_perm
+  (ts0: heap_elems_wf_ts) (s0: tree_id_seq ts0)
+  (ts1: heap_elems_wf_ts) (s1: tree_id_seq ts1): Lemma
+  (requires ts0.forest == ts1.forest /\ permutation U32.t s0 s1)
+  (ensures forest_freq ts0 s0 == forest_freq ts1 s1)
+  (decreases length s0) =
+  perm_len s0 s1;
+  if length s0 > 0 then
+    let i = index_of s1 s0.[0] in
+    calc (==) {
+      forest_freq ts0 s0;
+      =={}
+      freq ts1.forest.[U32.v s1.[i]] + forest_freq ts0 (tail s0);
+      =={
+        permutation_middle s0 s1;
+        lemma_forest_freq_perm
+          ts0 (tail s0)
+          ts1 (slice s1 0 i @| slice s1 (i + 1) (length s1))
+      }
+      freq ts1.forest.[U32.v s1.[i]] +
+      forest_freq ts1 (slice s1 0 i @| slice s1 (i + 1) (length s1));
+      =={lemma_forest_freq_append ts1 (slice s1 0 i) (slice s1 (i + 1) (length s1))}
+      freq ts1.forest.[U32.v s1.[i]] +
+      forest_freq ts1 (slice s1 0 i) +
+      forest_freq ts1 (slice s1 (i + 1) (length s1));
+      =={lemma_forest_freq_middle ts1 s1 i}
+      forest_freq ts1 s1;
+    }
+#pop-options
+
+#push-options "--fuel 0 --ifuel 0"
+let lemma_pqremove_forest ts node =
+  let ts' = pqremove ts in
+  let s = intermediate_fseq ts' in
+  let open FStar.Classical in
+  lemma_pqremove_id ts node;
+  forall_intro (lemma_pqremove_forest' ts);
+
+  lemma_heap_seq_tree_index ts;
+  lemma_intermediate_fseq_tree_index ts';
+
+  lemma_forest_symbols_perm ts (heap_seq ts) ts' s;
+  lemma_forest_freq_perm ts (heap_seq ts) ts' s
+#pop-options
+
+#push-options "--fuel 1 --ifuel 1"
+let rec lemma_forest_freq_plus_aux
+  (ts: heap_elems_wf_ts) (s: tree_id_seq ts) (i j: index_t s): Lemma
+  (requires
+    i <> j /\
+    length s > 1 /\
+    heap_not_empty ts /\
+    (forall k. freq_corr ts k) /\
+    (forall k. mem s.[k] (element_seq ts)))
+  (ensures
+    U16.v (ts.tree.[U32.v s.[i]]).freq_or_code +
+    U16.v (ts.tree.[U32.v s.[j]]).freq_or_code <=
+    forest_freq ts s)
+  (decreases i) =
+  let min = if i < j then i else j in
+  let max = if i < j then j else i in
+  let fi = U16.v (ts.tree.[U32.v s.[i]]).freq_or_code in
+  let fj = U16.v (ts.tree.[U32.v s.[j]]).freq_or_code in
+  let m1 = U16.v (ts.tree.[U32.v s.[min]]).freq_or_code in
+  let m2 = U16.v (ts.tree.[U32.v s.[max]]).freq_or_code in
+  match min with
+  | 0 ->
+    calc (<=) {
+      fi + fj;
+      =={}
+      m1 + m2;
+      <={}
+      m1 + forest_freq ts (slice (tail s) 0 (max - 1)) +
+      m2 + forest_freq ts (slice (tail s) max (length (tail s)));
+      =={
+        mem_index (tail s).[max - 1] (element_seq ts);
+        assert(exists (j: heap_index ts). ts.heap.[j] == s.[max])
+      }
+      m1 +
+      (forest_freq ts (slice (tail s) 0 (max - 1)) +
+      freq ts.forest.[U32.v (tail s).[max - 1]] +
+      forest_freq ts (slice (tail s) max (length (tail s))));
+      =={lemma_forest_freq_middle ts (tail s) (max - 1)}
+      m1 + forest_freq ts (tail s);
+      =={
+        mem_index s.[0] (element_seq ts);
+        assert(exists (j: heap_index ts). ts.heap.[j] == s.[min])
+      }
+      forest_freq ts s;
+    }
+  | _ -> lemma_forest_freq_plus_aux ts (tail s) (i - 1) (j - 1)
+#pop-options
+
+let lemma_forest_freq_plus ts i j =
+  let es = element_seq ts in
+  let s = cons ts.heap.[ts.heap_max] (heap_seq ts) in
+  assert(s.[0] == es.[ts.heap_len]);
+  assert(forall k. {:pattern s.[k]} k > 0 ==> s.[k] == es.[k - 1]);
+  assert(forall k. mem s.[k] (element_seq ts));
+  lemma_forest_freq_plus_aux ts s i j
+
+let rec fs_begin (ts: heap_elems_wf_ts) (s: tree_id_seq ts) (i: index_t s):
+  Tot nat (decreases i) =
+  match i with
+  | 0 -> 0
+  | _ ->
+    length (symbols ts.forest.[U32.v s.[0]]) + fs_begin ts (tail s) (i - 1)
+
+let rec fs_end (ts: heap_elems_wf_ts) (s: tree_id_seq ts) (i: index_t s):
+  Tot (res: nat{res <= length (forest_symbols ts s)}) (decreases i) =
+  match i with
+  | 0 -> length (symbols ts.forest.[U32.v s.[0]])
+  | _ -> length (symbols ts.forest.[U32.v s.[0]]) + fs_end ts (tail s) (i - 1)
+
+#push-options "--fuel 1 --ifuel 1"
+let rec lemma_symbols_length_gt_zero (t: tree): Lemma
+  (ensures length (symbols t) > 0)
+  [SMTPat (length (symbols t))] =
+  match t with
+  | Node l _ _ r ->
+    lemma_symbols_length_gt_zero l;
+    lemma_symbols_length_gt_zero r
+  | Leaf s _ -> ()
+
+let rec lemma_fs_begin_lt_end_1
+  (ts: heap_elems_wf_ts) (s: tree_id_seq ts) (i: index_t s): Lemma
+  (ensures fs_begin ts s i < fs_end ts s i)
+  (decreases i)
+  [SMTPat (fs_begin ts s i); SMTPat (fs_end ts s i)] =
+  match i with
+  | 0 -> ()
+  | _ -> lemma_fs_begin_lt_end_1 ts (tail s) (i - 1)
+
+let rec lemma_fs_begin_lt_end_2
+  (ts: heap_elems_wf_ts) (s: tree_id_seq ts) (i j: index_t s): Lemma
+  (requires i < j)
+  (ensures fs_end ts s i <= fs_begin ts s j)
+  (decreases i)
+  [SMTPat (fs_end ts s i); SMTPat (fs_begin ts s j)] =
+  match i with
+  | 0 -> ()
+  | _ -> lemma_fs_begin_lt_end_2 ts (tail s) (i - 1) (j - 1)
+
+let rec lemma_fs_begin_ascending
+  (ts: heap_elems_wf_ts) (s: tree_id_seq ts) (i j: index_t s): Lemma
+  (requires i < j)
+  (ensures fs_begin ts s i < fs_begin ts s j)
+  (decreases i)
+  [SMTPat (fs_begin ts s i); SMTPat (fs_begin ts s j)] =
+  match i with
+  | 0 -> ()
+  | _ -> lemma_fs_begin_ascending ts (tail s) (i - 1) (j - 1)
+
+let rec lemma_fs_end_ascending
+  (ts: heap_elems_wf_ts) (s: tree_id_seq ts) (i j: index_t s): Lemma
+  (requires i < j)
+  (ensures fs_end ts s i < fs_end ts s j)
+  (decreases i)
+  [SMTPat (fs_end ts s i); SMTPat (fs_end ts s j)] =
+  match i with
+  | 0 ->
+    calc (<) {
+      0;
+      <{}
+      length (symbols ts.forest.[U32.v s.[0]]);
+      =={}
+      fs_end ts s i;
+      <{}
+      length (symbols ts.forest.[U32.v s.[0]]) + fs_end ts (tail s) (j - 1);
+    }
+  | _ -> lemma_fs_end_ascending ts (tail s) (i - 1) (j - 1)
+
+let rec lemma_fs_slice (ts: heap_elems_wf_ts) (s: tree_id_seq ts) (i: index_t s): Lemma
+  (ensures
+    slice (forest_symbols ts s) (fs_begin ts s i) (fs_end ts s i) ==
+    symbols ts.forest.[U32.v s.[i]])
+  (decreases i) =
+  let a = slice (forest_symbols ts s) (fs_begin ts s i) (fs_end ts s i) in
+  let a' = symbols ts.forest.[U32.v s.[i]] in
+  match i with
+  | 0 -> assert(a `equal` a')
+  | _ ->
+    let hd = symbols ts.forest.[U32.v s.[0]] in
+    calc (==) {
+      slice (forest_symbols ts s) (fs_begin ts s i) (fs_end ts s i);
+      =={}
+      slice
+        (hd @| forest_symbols ts (tail s))
+        (length hd + fs_begin ts (tail s) (i - 1))
+        (length hd + fs_end ts (tail s) (i - 1));
+      =={append_slices hd (forest_symbols ts (tail s))}
+      slice
+        (forest_symbols ts (tail s))
+        (fs_begin ts (tail s) (i - 1))
+        (fs_end ts (tail s) (i - 1));
+      =={lemma_fs_slice ts (tail s) (i - 1)}
+      symbols ts.forest.[U32.v (tail s).[i - 1]];
+      =={}
+      symbols ts.forest.[U32.v s.[i]];
+    }
+
+#push-options "--z3rlimit 1024 --fuel 0 --ifuel 0"
+let lemma_pqmerge_disjoint' (ts: heap_elems_wf_ts) (i j: pos): Lemma
+  (requires
+    pqmerge_no_dup_pre ts i j /\
+    ((i < j /\ j <> ts.heap_max) \/ i == ts.heap_max))
+  (ensures (
+    let i' = U32.v ts.heap.[i] in
+    let j' = U32.v ts.heap.[j] in
+    no_dup (symbols ts.forest.[i']) /\
+    no_dup (symbols ts.forest.[j']) /\
+    disjoint (symbols ts.forest.[i']) (symbols ts.forest.[j'])
+  )) =
+  let cs = cons ts.heap.[ts.heap_max] (heap_seq ts) in
+  let ci = if i = ts.heap_max then 0 else i in
+  let cj = if j = ts.heap_max then 0 else j in
+  let fs = forest_symbols ts cs in
+  let bi = fs_begin ts cs ci in let ei = fs_end ts cs ci in
+  let bj = fs_begin ts cs cj in let ej = fs_end ts cs cj in
+  let fs' = slice fs bi ej in
+  lemma_fs_slice ts cs ci;
+  lemma_fs_slice ts cs cj;
+  no_dup_slice fs bi ej;
+  no_dup_slice fs' (ei - bi) (bj - bi)
+
+let lemma_pqmerge_no_dup ts i j =
+  if i < j && j <> ts.heap_max || i = ts.heap_max then
+    lemma_pqmerge_disjoint' ts i j
+  else
+    lemma_pqmerge_disjoint' ts j i
+
+let lemma_pqmerge_heap_wf
+  (ts: heap_wf_ts) (node: nat) (ts': tree_state_wf) (t': wf_tree): Lemma
+  (requires pqmerge_main_pre ts node ts' t')
+  (ensures heap_elems_wf ts') = ()
+
+#push-options "--query_stats"
+let lemma_pqmerge_smaller_heap
+  (ts: heap_wf_ts) (node: nat) (ts': tree_state_wf) (t': wf_tree)
+  (i j: pos): Lemma
+  (requires
+    pqmerge_main_pre ts node ts' t' /\
+    2 <= i /\ 2 <= j /\ i <= ts'.heap_len /\ j <= ts'.heap_len)
+  (ensures (
+    lemma_pqmerge_heap_wf ts node ts' t';
+    smaller ts' ts'.heap.[i] ts'.heap.[j] ==
+    smaller ts ts.heap.[i] ts.heap.[j])) =
+  let es = element_seq ts in
+  assert(forall i. id ts.forest.[U32.v es.[i]] == U32.v es.[i]);
+  assert(forall i. 2 <= i /\ i <= ts.heap_len ==>
+    es.[i - 1] == ts.heap.[i] /\ ts'.heap.[i] == ts.heap.[i]);
+  assert(forall i. 2 <= i /\ i <= ts'.heap_len ==> U32.v ts'.heap.[i] < node);
+  assert(forall i. i <> node ==> (ts'.tree.[i]).freq_or_code == (ts.tree.[i]).freq_or_code)
+
+let lemma_pqmerge_smaller_sorted
+  (ts: heap_wf_ts) (node: nat) (ts': tree_state_wf) (t': wf_tree)
+  (i j: pos): Lemma
+  (requires
+    pqmerge_main_pre ts node ts' t' /\
+    ts'.heap_max < i /\ ts'.heap_max < j /\
+    i < U32.v heap_size /\ j < U32.v heap_size)
+  (ensures (
+    lemma_pqmerge_heap_wf ts node ts' t';
+    smaller ts' ts'.heap.[i] ts'.heap.[j] ==
+    smaller ts ts.heap.[i] ts.heap.[j])) =
+  let es = element_seq ts in
+  assert(forall i. id ts.forest.[U32.v es.[i]] == U32.v es.[i]);
+  assert(forall i. ts.heap_max <= i /\ i <= U32.v heap_size ==>
+    es.[i - ts.heap_max + ts.heap_len] == ts.heap.[i] /\ ts'.heap.[i] == ts.heap.[i]);
+  assert(forall i. ts.heap_max <= i /\ i <= U32.v heap_size ==> U32.v ts'.heap.[i] < node);
+  assert(forall i. i <> node ==> (ts'.tree.[i]).freq_or_code == (ts.tree.[i]).freq_or_code)
+
+#push-options "--fuel 1 --ifuel 1"
+let rec lemma_pqmerge_heap_sorted_aux
+  (ts: heap_wf_ts) (node: nat) (ts': tree_state_wf) (t': wf_tree) (i: nat): Lemma
+  (requires
+    pqmerge_main_pre ts node ts' t' /\
+    ts.heap_max <= i /\ i <= U32.v heap_size)
+  (ensures heap_sorted' ts i)
+  (decreases i - ts.heap_max) =
+  if ts.heap_max < i then lemma_pqmerge_heap_sorted_aux ts node ts' t' (i - 1)
+
+let rec lemma_pqmerge_heap_sorted
+  (ts: heap_wf_ts) (node: nat) (ts': heap_elems_wf_ts) (t': wf_tree) (i: nat): Lemma
+  (requires
+    pqmerge_main_pre ts node ts' t' /\
+    ts'.heap_max <= i /\ i <= U32.v heap_size)
+  (ensures heap_sorted' ts' i)
+  (decreases U32.v heap_size - i) = 
+  if U32.v heap_size - i <= 1 then
+    ()
+  else if ts'.heap_max < i then begin
+    lemma_pqmerge_heap_sorted_aux ts node ts' t' i;
+    lemma_pqmerge_heap_sorted ts node ts' t' (i + 1);
+    lemma_pqmerge_smaller_sorted ts node ts' t' (i + 1) i
+  end else begin
+    let k = ts.heap.[ts.heap_max] in
+    let l = ts.heap.[1] in
+    let es = element_seq ts in
+    assert(es.[ts.heap_len] == k /\ es.[0] == l);
+    lemma_pqmerge_heap_sorted ts node ts' t' (i + 1)
+  end
+#pop-options
+
+let lemma_pqmerge_partial_wf
+  (ts: heap_wf_ts) (node: nat) (ts': heap_elems_wf_ts) (t': wf_tree)
+  (i: pos{2 <= i /\ i <= ts'.heap_len / 2}): Lemma
+  (requires pqmerge_main_pre ts node ts' t')
+  (ensures
+    smaller ts' ts'.heap.[i] ts'.heap.[i * 2] /\
+    (i * 2 + 1 <= ts'.heap_len ==> smaller ts' ts'.heap.[i] ts'.heap.[i * 2 + 1])) =
+  lemma_pqmerge_smaller_heap ts node ts' t' i (i * 2);
+  if i * 2 + 1 <= ts'.heap_len then
+    lemma_pqmerge_smaller_heap ts node ts' t' i (i * 2 + 1)
+
+let lemma_pqmerge_sorted_lt_heap 
+  (ts: heap_wf_ts) (node: nat) (ts': heap_elems_wf_ts) (t': wf_tree)
+  (i: pos{i <= ts'.heap_len}): Lemma
+  (requires pqmerge_main_pre ts node ts' t' /\ sorted_not_empty ts')
+  (ensures smaller ts' ts'.heap.[ts'.heap_max] ts'.heap.[i]) =
+  let hd = U32.v ts'.heap.[ts'.heap_max] in
+  let r = U32.v ts'.heap.[i] in
+  let es = element_seq ts in
+  assert(U32.v es.[0] == hd);
+  if 1 < i then begin
+    assert(U32.v es.[i - 1] == r);
+    lemma_heap_wf ts i
+  end else begin
+    let hd' = U32.v ts'.heap.[ts'.heap_max + 1] in
+    assert(freq_corr ts ts.heap_max);
+    assert(U16.v (ts'.tree.[hd]).freq_or_code == freq ts'.forest.[hd]);
+    assert(U16.v (ts'.tree.[hd']).freq_or_code == freq ts'.forest.[hd']);
+    assert(U16.v (ts'.tree.[r]).freq_or_code > U16.v (ts'.tree.[hd]).freq_or_code)
+  end
+
+let lemma_pqmerge_max_id
+  (ts: heap_wf_ts) (node: nat) (ts': heap_elems_wf_ts) (t': wf_tree)
+  (i: nat{i < ts'.heap_len - 1}): Lemma
+  (requires pqmerge_main_pre ts node ts' t')
+  (ensures U32.v (tail (heap_seq ts')).[i] < node) =
+  let tl = tail (heap_seq ts') in
+  assert(tl.[i] == (heap_seq ts).[i + 1] /\ tl.[i] == (element_seq ts).[i + 1])
+
+#push-options "--z3seed 2 --fuel 1 --ifuel 1"
+let rec lemma_pqmerge_forest_symbols_aux
+  (ts: heap_wf_ts) (node: nat) (ts': heap_elems_wf_ts) (t': wf_tree)
+  (s: tree_id_seq ts'): Lemma
+  (requires
+    pqmerge_main_pre ts node ts' t' /\
+    (forall i. U32.v s.[i] < node))
+  (ensures forest_symbols ts s == forest_symbols ts' s)
+  (decreases length s) =
+  match length s with
+  | 0 -> ()
+  | _ -> lemma_pqmerge_forest_symbols_aux ts node ts' t' (tail s)
+
+let lemma_pqmerge_forest_symbols
+  (ts: heap_wf_ts) (node: nat) (ts': heap_elems_wf_ts) (t': wf_tree): Lemma
+  (requires pqmerge_main_pre ts node ts' t')
+  (ensures forest_symbols ts (intermediate_fseq ts) == forest_symbols ts' (heap_seq ts')) =
+  let open FStar.Classical in
+  let tl = tail (heap_seq ts') in
+  calc (==) {
+    forest_symbols ts (intermediate_fseq ts);
+    ={lemma_forest_symbols_append ts (create 1 ts.heap.[ts.heap_max]) (heap_seq ts)}
+    forest_symbols ts (create 1 ts.heap.[ts.heap_max]) @|
+    forest_symbols ts (heap_seq ts);
+    =={lemma_forest_symbols_single ts ts.heap.[ts.heap_max]}
+    symbols ts.forest.[U32.v ts.heap.[ts.heap_max]] @|
+    forest_symbols ts (heap_seq ts);
+    =={}
+    symbols ts.forest.[U32.v ts.heap.[ts.heap_max]] @|
+    (symbols ts.forest.[U32.v ts.heap.[1]] @|
+    forest_symbols ts (tail (heap_seq ts)));
+    =={
+      append_assoc
+        (symbols ts.forest.[U32.v ts.heap.[ts.heap_max]])
+        (symbols ts.forest.[U32.v ts.heap.[1]])
+        (forest_symbols ts (tail (heap_seq ts)))
+    }
+    (symbols ts.forest.[U32.v ts.heap.[ts.heap_max]] @|
+    symbols ts.forest.[U32.v ts.heap.[1]]) @|
+    forest_symbols ts (tail (heap_seq ts));
+    =={}
+    (symbols ts'.forest.[U32.v ts'.heap.[ts.heap_max]] @|
+    symbols ts'.forest.[U32.v ts'.heap.[ts'.heap_max]]) @|
+    forest_symbols ts (tail (heap_seq ts));
+    =={assert((tail (heap_seq ts)) `equal` tl)}
+    (symbols ts'.forest.[U32.v ts'.heap.[ts.heap_max]] @|
+    symbols ts'.forest.[U32.v ts'.heap.[ts'.heap_max]]) @|
+    forest_symbols ts tl;
+    =={
+      forall_intro (move_requires (lemma_pqmerge_max_id ts node ts' t'));
+      lemma_pqmerge_forest_symbols_aux ts node ts' t' tl
+    }
+    (symbols ts'.forest.[U32.v ts'.heap.[ts.heap_max]] @|
+    symbols ts'.forest.[U32.v ts'.heap.[ts'.heap_max]]) @|
+    forest_symbols ts' tl;
+    =={}
+    symbols t' @| forest_symbols ts' tl;
+    =={}
+    forest_symbols ts' (heap_seq ts');
+  }
+
+let rec lemma_pqmerge_forest_freq_aux
+  (ts: heap_wf_ts) (node: nat) (ts': heap_elems_wf_ts) (t': wf_tree)
+  (s: tree_id_seq ts'): Lemma
+  (requires
+    pqmerge_main_pre ts node ts' t' /\
+    (forall i. U32.v s.[i] < node))
+  (ensures forest_freq ts s == forest_freq ts' s)
+  (decreases length s) =
+  match length s with
+  | 0 -> ()
+  | _ -> lemma_pqmerge_forest_freq_aux ts node ts' t' (tail s)
+#pop-options
+
+#push-options "--fuel 2 --ifuel 2"
+let lemma_forest_freq_single
+  (ts: heap_elems_wf_ts) (s: U32.t{is_tree_index ts s}): Lemma
+  (ensures freq ts.forest.[U32.v s] == forest_freq ts (create 1 s)) = ()
+#pop-options
+
+#push-options "--z3seed 7 --fuel 1 --ifuel 0"
+let lemma_pqmerge_forest_freq
+  (ts: heap_wf_ts) (node: nat) (ts': heap_elems_wf_ts) (t': wf_tree): Lemma
+  (requires pqmerge_main_pre ts node ts' t')
+  (ensures forest_freq ts (intermediate_fseq ts) == forest_freq ts' (heap_seq ts')) =
+  let open FStar.Classical in
+  let tl = tail (heap_seq ts') in
+  calc (==) {
+    forest_freq ts (intermediate_fseq ts);
+    =={}
+    forest_freq ts (create 1 ts.heap.[ts.heap_max] @| heap_seq ts);
+    =={lemma_forest_freq_append ts (create 1 ts.heap.[ts.heap_max]) (heap_seq ts)}
+    forest_freq ts (create 1 ts.heap.[ts.heap_max]) + forest_freq ts (heap_seq ts);
+    =={lemma_tl ts.heap.[1] (tail (heap_seq ts))}
+    forest_freq ts (create 1 ts.heap.[ts.heap_max]) +
+    forest_freq ts (create 1 ts.heap.[1] @| tail (heap_seq ts));
+    =={lemma_forest_freq_append ts (create 1 ts.heap.[1]) (tail (heap_seq ts))}
+    forest_freq ts (create 1 ts.heap.[ts.heap_max]) +
+    forest_freq ts (create 1 ts.heap.[1]) +
+    forest_freq ts (tail (heap_seq ts));
+    =={
+      lemma_forest_freq_single ts ts.heap.[1];
+      lemma_forest_freq_single ts ts.heap.[ts.heap_max]
+    }
+    freq ts.forest.[U32.v ts.heap.[ts.heap_max]] +
+    freq ts.forest.[U32.v ts.heap.[1]] +
+    forest_freq ts (tail (heap_seq ts));
+    =={}
+    freq t' + forest_freq ts (tail (heap_seq ts));
+    =={assert((tail (heap_seq ts)) `equal` tl)}
+    freq t' + forest_freq ts (tail (heap_seq ts'));
+    =={
+      forall_intro (move_requires (lemma_pqmerge_max_id ts node ts' t'));
+      lemma_pqmerge_forest_freq_aux ts node ts' t' tl
+    }
+    freq t' + forest_freq ts' (tail (heap_seq ts'));
+    =={}
+    forest_freq ts' (heap_seq ts');
+  }
+#pop-options
+
+#push-options "--z3seed 0 --fuel 1 --ifuel 1"
+let lemma_pqmerge_count_aux_1
+  (ts: heap_wf_ts) (node: nat) (ts': heap_elems_wf_ts) (t': wf_tree): Lemma
+  (requires pqmerge_main_pre ts node ts' t')
+  (ensures (
+    let es = element_seq ts in
+    let es' = element_seq ts' in
+    U32.v es'.[0] == node /\
+    (forall i.{:pattern es'.[i]} 1 <= i /\ i < ts.heap_len ==> es.[i] == es'.[i]) /\
+    es'.[ts.heap_len] == es.[0] /\
+    (forall i.{:pattern es'.[i]} ts.heap_len + 1 <= i ==> es'.[i] == es.[i - 1]) /\
+    (forall i.{:pattern es.[i]} id ts.forest.[U32.v es.[i]] == U32.v es.[i]) /\
+
+    (forall i. {:pattern es.[i]} U32.v es.[i] < node) /\
+    (forall i. {:pattern es'.[i]} 1 < i ==> U32.v es'.[i] < node))) =
+  let es = element_seq ts in
+  let es' = element_seq ts' in
+  assert(U32.v es'.[0] == node);
+  assert(forall i.{:pattern es'.[i]} 1 <= i /\ i < ts.heap_len ==> es.[i] == es'.[i]);
+  assert(es'.[ts.heap_len] == es.[0]);
+  assert(forall i.{:pattern es'.[i]} ts.heap_len + 1 <= i ==> es'.[i] == es.[i - 1]);
+  assert(forall i.{:pattern es.[i]} id ts.forest.[U32.v es.[i]] == U32.v es.[i]);
+  assert(no_dup es);
+  assert(forall i. {:pattern es.[i]} U32.v es.[i] < node);
+  assert(forall i. {:pattern es'.[i]} 1 < i ==> U32.v es'.[i] < node)
+#pop-options
+
+#push-options "--z3seed 0 --fuel 0 --ifuel 0"
+let lemma_pqmerge_count_aux_2
+  (ts: heap_wf_ts) (node: nat) (ts': heap_elems_wf_ts) (t': wf_tree): Lemma
+  (requires pqmerge_main_pre ts node ts' t')
+  (ensures (
+    let es = element_seq ts in
+    let es' = element_seq ts' in
+    tail es' `equal` (slice es 1 ts.heap_len @| create 1 es.[0] @| sorted_seq ts))) =
+  lemma_pqmerge_count_aux_1 ts node ts' t'
+#pop-options
+
+#push-options "--z3seed 0 --fuel 1 --ifuel 0"
+let lemma_pqmerge_count
+  (ts: heap_wf_ts) (node: nat) (ts': heap_elems_wf_ts) (t': wf_tree)
+  (n: U32.t): Lemma
+  (requires pqmerge_main_pre ts node ts' t')
+  (ensures (
+    let es = element_seq ts in
+    let es' = element_seq ts' in
+    (U32.v n == node ==> count n es' == 1 /\ mem n es == false) /\
+    (U32.v n <> node ==> count n es' == count n es))) =
+  let es = element_seq ts in
+  let es' = element_seq ts' in
+  if U32.v n = node then begin
+    lemma_pqmerge_count_aux_1 ts node ts' t';
+    if mem n es then mem_index n es;
+    if mem n (tail es') then mem_index n (tail es');
+    calc (==) {
+      count n es';
+      =={}
+      1 + count n (tail es');
+    }
+  end else
+    calc (==) {
+      count n es';
+      =={}
+      count n (tail es');
+      =={lemma_pqmerge_count_aux_2 ts node ts' t'}
+      count n (slice es 1 ts.heap_len @| create 1 es.[0] @| sorted_seq ts);
+      =={append_assoc (slice es 1 ts.heap_len) (create 1 es.[0]) (sorted_seq ts)}
+      count n ((slice es 1 ts.heap_len @| create 1 es.[0]) @| sorted_seq ts);
+      =={
+        lemma_append_count (slice es 1 ts.heap_len @| create 1 es.[0]) (sorted_seq ts)
+      }
+      count n (slice es 1 ts.heap_len @| create 1 es.[0]) + count n (sorted_seq ts);
+      =={lemma_append_count (slice es 1 ts.heap_len) (create 1 es.[0])}
+      count n (create 1 es.[0]) +
+      count n (slice es 1 ts.heap_len) +
+      count n (sorted_seq ts);
+      =={lemma_append_count (create 1 es.[0]) (slice es 1 ts.heap_len)}
+      count n (create 1 es.[0] @| slice es 1 ts.heap_len) + count n (sorted_seq ts);
+      =={
+        calc (==) {
+          slice es 1 ts.heap_len;
+          =={}
+          slice (slice es 0 ts.heap_len) 1 ts.heap_len;
+          =={assert((slice es 0 ts.heap_len) `equal` (heap_seq ts))}
+          tail (heap_seq ts);
+        }
+      }
+      count n (create 1 es.[0] @| tail (heap_seq ts)) + count n (sorted_seq ts);
+      =={assert((create 1 es.[0] @| tail (heap_seq ts)) `equal` heap_seq ts)}
+      count n (heap_seq ts) + count n (sorted_seq ts);
+      =={lemma_append_count (heap_seq ts) (sorted_seq ts)}
+      count n (heap_seq ts @| sorted_seq ts);
+      =={}
+      count n es;
+    }
+#pop-options
+
+let lemma_pqmerge_id_max
+  (ts: heap_wf_ts) (node: nat) (ts': heap_elems_wf_ts{
+    heap_not_empty ts'
+  }) (t': wf_tree) (i: nat{
+    i < length (element_seq ts')
+  }) : Lemma
+  (requires pqmerge_main_pre ts node ts' t')
+  (ensures id ts'.forest.[U32.v (element_seq ts').[i]] < node + 1) =
+  let open FStar.Classical in
+  let es = element_seq ts in
+  let es' = element_seq ts' in
+  if i = 0 then
+    assert(id ts'.forest.[U32.v es'.[i]] == node)
+  else begin
+    forall_intro (move_requires (lemma_pqmerge_count ts node ts' t'));
+    no_dup_alt es' i 0;
+    mem_index es'.[i] es
+  end
+
+#push-options "--fuel 2 --ifuel 2"
+let lemma_pqmerge_child_corr
+  (ts: heap_wf_ts) (node: nat) (ts': heap_elems_wf_ts) (t': wf_tree)
+  (i: heap_index ts'): Lemma
+  (requires pqmerge_main_pre ts node ts' t')
+  (ensures child_corr ts' i) =
+  let open FStar.Classical in
+  let es = element_seq ts in
+  let es' = element_seq ts' in
+  if i = 1 || i = ts'.heap_max then
+    admit()
+  else begin
+    let i' = U32.v ts.heap.[i] in
+    let t = ts.forest.[i'] in
+    assert(ts.heap.[i] == ts'.heap.[i]);
+    assume(i' < node);
+    assert(t == ts'.forest.[i']);
+    if Node? t then begin
+      assert(id t < node);
+      assert(id (left t) < id t /\ id (right t) < id t);
+      assert((ts.tree.[id (left t)]).dad_or_len == (ts'.tree.[id (left t)]).dad_or_len);
+      assume((ts.tree.[id (right t)]).dad_or_len == (ts'.tree.[id (right t)]).dad_or_len);
+      assert(ts.forest.[id (left t)] == ts'.forest.[id (left t)]);
+      assert(ts.forest.[id (right t)] == ts'.forest.[id (right t)]);
+      assume(id ts'.forest.[U32.v ts'.heap.[i]] == U32.v ts'.heap.[i])
+    end;
+    assume(id ts'.forest.[U32.v ts'.heap.[i]] == U32.v ts'.heap.[i]);
+    assert(1 <= i /\ i <= ts.heap_len \/ ts.heap_max <= i /\ i < U32.v heap_size);
+    assert(child_corr ts' i);
+    admit()
+  end
+
+let lemma_pqmerge_main ts node ts' t' =
+  let open FStar.Classical in
+  lemma_pqmerge_heap_wf ts node ts' t';
+  lemma_pqmerge_heap_sorted ts node ts' t' ts'.heap_max;
+  forall_intro (move_requires (lemma_pqmerge_partial_wf ts node ts' t'));
+  forall_intro (move_requires (lemma_pqmerge_sorted_lt_heap ts node ts' t'));
+  lemma_pqmerge_forest_symbols ts node ts' t';
+  lemma_pqmerge_forest_freq ts node ts' t';
+  forall_intro (move_requires (lemma_pqmerge_count ts node ts' t'));
+  forall_intro (move_requires (lemma_pqmerge_id_max ts node ts' t'));
+  forall_intro (move_requires (lemma_pqmerge_child_corr ts node ts' t'))
