specs/Spec.Tree.fst
@@ -1,0 +1,122 @@
+module Spec.Tree
+
+module U8 = FStar.UInt8
+module U16 = FStar.UInt16
+module U32 = FStar.UInt32
+
+open FStar.Seq
+open Lib.Seq
+open Spec.Heap
+open Yazi.Tree.Types
+include Spec.Tree.Lemmas
+
+/// Merge two trees that have the lowest frequencies after the call of pqremove.
+#push-options "--z3refresh --z3rlimit 1024 --fuel 1 --ifuel 1"
+let pqmerge (ts: heap_wf_ts) (node: nat): Pure tree_state_wf
+  (requires pqmerge_pre ts node)
+  (ensures fun ts' -> pqmerge_post ts node ts') =
+  let il = U32.v ts.heap.[ts.heap_max] in
+  let hl = U8.v ts.depth.[il] in
+  let l = ts.forest.[il] in
+  let t1 = ts.tree.(il) <- ({
+    (ts.tree).[il] with
+    dad_or_len = U16.uint_to_t node;
+  }) in
+ 
+  let ir = U32.v ts.heap.[1] in
+  let hr = U8.v ts.depth.[ir] in
+  let r = ts.forest.[ir] in
+  let t2 = t1.(ir) <- ({
+    (ts.tree).[ir] with
+    dad_or_len = U16.uint_to_t node;
+  }) in
+
+  let t' = Node l node (freq l + freq r) r in
+  lemma_is_max_id_map ts node 1;
+  lemma_is_max_id_map ts node ts.heap_max;
+  lemma_pqmerge_no_dup ts ts.heap_max 1;
+
+  let dt' = (1 + (if hl >= hr then hl else hr)) % pow2 8 in
+
+  lemma_forest_freq_plus ts 0 1;
+  let t3 = t2.(node) <- ({
+    t2.[node] with
+    freq_or_code = (t2.[il]).freq_or_code `U16.add` (t2.[ir]).freq_or_code;
+  }) in
+
+  let heap_max' = ts.heap_max - 1 in
+  let heap' = ts.heap.(heap_max') <- U32.uint_to_t ir in
+  let heap'' = heap'.(1) <- U32.uint_to_t node in
+  let ts': tree_state_wf = {
+    ts with
+    heap = heap'';
+    heap_max = heap_max';
+    forest = ts.forest.(node) <- t';
+    depth = ts.depth.(node) <- U8.uint_to_t dt';
+    tree = t3;
+  } in
+  lemma_pqmerge_main ts node ts' t';
+  admit();
+  ts'
+
+#push-options "--z3refresh --z3rlimit 1024 --fuel 1 --ifuel 1"
+/// Merge the two trees that have the lowest frequencies.
+let merge_tree (ts: forest_wf_ts) (node: nat):
+  Ghost forest_wf_ts
+  (requires
+    ts.heap_len > 1 /\
+    // (forall i. i >= node ==> U8.v (ts.depth).[i] == 0) /\
+    is_max_id ts node)
+  (ensures fun ts' ->
+    ts' == {
+      ts with
+      heap = ts'.heap;
+      heap_len = ts.heap_len - 1;
+      heap_max = ts.heap_max - 2;
+      forest = ts'.forest;
+      depth = ts'.depth;
+      tree = ts'.tree;
+    } /\
+    (forall s. U32.v s <> node ==>
+      count s (element_seq ts) == count s (element_seq ts')) /\
+    count (U32.uint_to_t node) (element_seq ts') == 1 /\
+    permutation nat (forest_symbols ts) (forest_symbols ts')) =
+  let ts' = pqremove ts in
+
+  let il = U32.v (ts'.heap).[ts'.heap_max] in
+  let hl = U8.v (ts'.depth).[il] in
+  let l = (ts'.forest).[il] in
+  let t1 = ts.tree.(il) <- ({
+    (ts.tree).[il] with
+    dad_or_len = U16.uint_to_t node;
+  }) in
+ 
+  let ir = U32.v (ts'.heap).[1] in
+  let hr = U8.v (ts'.depth).[ir] in
+  let r = (ts'.forest).[ir] in
+  let t2 = t1.(ir) <- ({
+    (ts.tree).[ir] with
+    dad_or_len = U16.uint_to_t node;
+  }) in
+ 
+  let t' = Node l node (freq l + freq r) r in
+  let dt' = (1 + (if hl >= hr then hl else hr)) % pow2 8 in
+  let t3 = t2.(node) <- ({
+    freq_or_code = (t2.[ir]).freq_or_code `U16.add` (t2.[ir]).freq_or_code;
+    dad_or_len = U16.uint_to_t node;
+  }) in
+  admit();
+  // lemma_wf_forest_symbols_disjoint ts' ts'.heap_max 1;
+
+  let heap_max' = ts'.heap_max - 1 in
+  let heap' = upd ts'.heap heap_max' (U32.uint_to_t ir) in
+ 
+  let ts'' = {
+    ts' with
+    heap = heap';
+    heap_max = heap_max';
+    forest = upd ts'.forest node t';
+    depth = ts'.depth.(node) <- (U8.uint_to_t dt');
+    tree = t3;
+  } in
+  pqdownheap ts'' 1ul
